books/kestrel/utilities/defevaluator-plus-tests.lisp
@@ -1,0 +1,20 @@
+; A nicer interface to defevaluator
+;
+; Copyright (C) 2014-2021 Kestrel Institute
+;
+; License: A 3-clause BSD license. See the file books/3BSD-mod.txt.
+;
+; Author: Eric Smith (eric.smith@kestrel.edu)
+
+;;;;;;;;;;;;;;;;;;;;;;;;;;;;;;;;;;;;;;;;;;;;;;;;;;;;;;;;;;;;;;;;;;;;;;;;;;;;;;;;
+
+(in-package "ACL2")
+
+(include-book "defevaluator-plus")
+(include-book "kestrel/utilities/deftest" :dir :system)
+
+(deftest
+  (defevaluator+ myev binary-*)
+  ;; expected result:
+  (must-be-redundant (defevaluator+ myev binary-*))
+  (defthm test (equal (myev '(binary-* '2 x) '((x . 3))) 6)))
